theories/TM/Reductions/Arbitrary_to_Binary.v
@@ -757,6 +757,7 @@ Proof.
   eapply TM_eval_iff in H as [k H].
   now eapply HM in H.
 Qed.
+
 Lemma Sim_Terminates {Σ} (L : finType) (M : pTM Σ L 1) T :
   projT1 M ↓ T ->
   exists C1 C2,
@@ -770,6 +771,35 @@ Proof.
   intros ? ? ?. TMSimp.
   eapply HM in H0. TMSimp. 
   destruct ymid1. destruct_tapes. repeat eexists; eassumption.
+Qed.
+
+Lemma binary_simulation Σ (M : TM Σ 1) :
+  {M' : TM (finType_CS bool) 1 |
+        (forall q t t', eval M (start M) t q t' -> exists q, eval M' (start M') ([| encode_tape' (Vector.nth t Fin0) |] ) q ([| encode_tape' (Vector.nth t' Fin0)  |] )) /\
+        (forall t, (exists q t', eval M' (start M') ([| encode_tape' (Vector.nth t Fin0) |] ) q t') -> (exists q t', eval M (start M) t q t')) }.
+Proof.
+  exists (projT1 (StateWhile (@Step Σ M) (start M))). split.
+  - intros q' t t' [n H] % TM_eval_iff.
+    edestruct @Sim_Terminates with (M := (existT _ M (fun _ : state M => tt))) (T := fun tin k => tin = t /\ k >= n).
+    * intros tin k [-> Hk]. cbn. exists (mk_mconfig q' t').  eapply @loop_monotone. exact H. eapply Hk.
+    * destruct H0 as [k H0]. cbn in H0. edestruct H0 as [[] H1].
+      -- exists (Vector.hd t), n. split. reflexivity. split. 2: now unfold ge. split. 2:lia.
+         destruct_tapes. reflexivity.
+      -- exists cstate. eapply TM_eval_iff. exists (x * n + k). unfold Relabel, initc in H1. cbn in H1.
+         destruct_tapes. etransitivity. exact H1.
+         cbn. repeat f_equal.
+         eapply (Sim_Realise (M := (existT _ M (fun _ : state M => tt))) (R := fun tin '(_,tout) => exists q', eval M (start M) tin q' tout)) in H1.
+         + destruct_tapes. rename h1 into t.
+           specialize (H1 t eq_refl) as [t'_sig [[q'_ [n' H1] % TM_eval_iff] H2]]. cbn in H1. 
+           cbn in H2. subst. inv H2. f_equal.
+           eapply loop_injective in H. 2: eassumption. now inv H.
+        + clear k H0 H1. intros tin k [q'_ tout] Hter. cbn in *. exists q'_. eapply TM_eval_iff. exists k. exact Hter.
+  - intros t (q' & t' & [n H] % TM_eval_iff). 
+    eapply (Sim_Realise (M := (existT _ M (fun _ : state M => tt))) (R := fun tin '(_,tout) => exists q', eval M (start M) tin q' tout)) in H.
+    * destruct_tapes. rename h0 into t.
+      specialize (H t eq_refl) as [t'_sig [[q'_ H1] H2]]. cbn in H1. 
+      cbn in H2. subst. exists q'_, [|t'_sig|]. eassumption. 
+    * intros tin k [q'_ tout] Hter. cbn in *. exists q'_. eapply TM_eval_iff. exists k. exact Hter.
 Qed.
 
 Require Import Undecidability.Synthetic.Definitions.
